Weidenbach_Book/IsaSAT_Trail.thy
@@ -1116,4 +1116,105 @@ lemma isa_length_trail_length_u_no_CS:
     (auto simp: isa_length_trail_def trail_pol_no_CS_alt_def ann_lits_split_reasons_def
       intro!: ASSERT_leI)
 
+
+lemma control_stack_is_decided:
+  \<open>control_stack cs M \<Longrightarrow> c\<in>set cs \<Longrightarrow> is_decided ((rev M)!c)\<close>
+  by (induction arbitrary: c rule: control_stack.induct) (auto simp: nth_append
+      dest: control_stack_le_length_M)
+
+lemma control_stack_distinct:
+  \<open>control_stack cs M \<Longrightarrow> distinct cs\<close>
+  by (induction rule: control_stack.induct) (auto simp: nth_append
+      dest: control_stack_le_length_M)
+
+lemma control_stack_level_control_stack:
+  assumes
+    cs: \<open>control_stack cs M\<close> and
+    n_d: \<open>no_dup M\<close> and
+    i: \<open>i < length cs\<close>
+  shows \<open>get_level M (lit_of (rev M ! (cs ! i))) = Suc i\<close>
+proof -
+  define L where \<open>L = rev M ! (cs ! i)\<close>
+  have csi: \<open>cs ! i < length M\<close>
+    using cs i by (auto intro: control_stack_le_length_M)
+  then have L_M: \<open>L \<in> set M\<close>
+    using nth_mem[of \<open>cs !i\<close> \<open>rev M\<close>] unfolding L_def by (auto simp del: nth_mem)
+  have dec_L: \<open>is_decided L\<close>
+    using control_stack_is_decided[OF cs] i unfolding L_def by auto
+  then have \<open>rev M!(cs ! (get_level M (lit_of L) - 1)) = L\<close>
+    using control_stack_rev_get_lev[OF cs n_d L_M] by auto
+  moreover have \<open>distinct M\<close>
+    using no_dup_distinct[OF n_d] unfolding mset_map[symmetric] distinct_mset_mset_distinct
+    by (rule distinct_mapI)
+
+  moreover have lev0:  \<open>get_level M (lit_of L) \<ge> 1\<close>
+    using split_list[OF L_M] n_d dec_L by (auto simp: get_level_append_if)
+  moreover have \<open>cs ! (get_level M (lit_of (rev M ! (cs ! i))) - Suc 0) < length M\<close>
+    using control_stack_le_length_M[OF cs,
+         of \<open>cs ! (get_level M (lit_of (rev M ! (cs ! i))) - Suc 0)\<close>, OF nth_mem]
+      control_stack_length_count_dec[OF cs] count_decided_ge_get_level[of M
+          \<open>lit_of (rev M ! (cs ! i))\<close>] lev0
+    by (auto simp: L_def)
+  ultimately have \<open>cs ! (get_level M (lit_of L) - 1) = cs ! i\<close>
+    using nth_eq_iff_index_eq[of \<open>rev M\<close>] csi unfolding L_def by auto
+  then have \<open>i = get_level M (lit_of L) - 1\<close>
+    using nth_eq_iff_index_eq[OF control_stack_distinct[OF cs], of i \<open>get_level M (lit_of L) - 1\<close>]
+      i lev0 count_decided_ge_get_level[of M \<open>lit_of (rev M ! (cs ! i))\<close>]
+    control_stack_length_count_dec[OF cs]
+    by (auto simp: L_def)
+  then show ?thesis using lev0 unfolding L_def[symmetric] by auto
+qed
+
+
+definition get_pos_of_level_in_trail where
+  \<open>get_pos_of_level_in_trail M\<^sub>0 lev =
+     SPEC(\<lambda>i. i < length M\<^sub>0 \<and> is_decided (rev M\<^sub>0!i) \<and> get_level M\<^sub>0 (lit_of (rev M\<^sub>0!i)) = lev+1)\<close>
+
+definition (in -) get_pos_of_level_in_trail_imp where
+  \<open>get_pos_of_level_in_trail_imp = (\<lambda>(M', xs, lvls, reasons, k, cs) lev. do {
+      ASSERT(lev < length cs);
+      RETURN (cs ! lev)
+   })\<close>
+definition get_pos_of_level_in_trail_pre where
+  \<open>get_pos_of_level_in_trail_pre = (\<lambda>(M, lev). lev < count_decided M)\<close>
+
+lemma get_pos_of_level_in_trail_imp_get_pos_of_level_in_trail:
+   \<open>(uncurry get_pos_of_level_in_trail_imp, uncurry get_pos_of_level_in_trail) \<in>
+    [get_pos_of_level_in_trail_pre]\<^sub>f trail_pol_no_CS \<A> \<times>\<^sub>f nat_rel \<rightarrow> \<langle>nat_rel\<rangle>nres_rel\<close>
+  apply (intro nres_relI frefI)
+  unfolding get_pos_of_level_in_trail_imp_def uncurry_def get_pos_of_level_in_trail_def
+    get_pos_of_level_in_trail_pre_def
+  apply clarify
+  apply (rule ASSERT_leI)
+  subgoal
+    by (auto simp: trail_pol_no_CS_alt_def dest!: control_stack_length_count_dec)
+  subgoal for a aa ab ac ad b ba ae bb
+    by (auto simp: trail_pol_no_CS_def control_stack_length_count_dec in_set_take_conv_nth
+        intro!: control_stack_le_length_M control_stack_is_decided
+        dest: control_stack_level_control_stack)
+  done
+
+lemma get_pos_of_level_in_trail_imp_get_pos_of_level_in_trail_CS:
+   \<open>(uncurry get_pos_of_level_in_trail_imp, uncurry get_pos_of_level_in_trail) \<in>
+    [get_pos_of_level_in_trail_pre]\<^sub>f trail_pol \<A> \<times>\<^sub>f nat_rel \<rightarrow> \<langle>nat_rel\<rangle>nres_rel\<close>
+  apply (intro nres_relI frefI)
+  unfolding get_pos_of_level_in_trail_imp_def uncurry_def get_pos_of_level_in_trail_def
+    get_pos_of_level_in_trail_pre_def
+  apply clarify
+  apply (rule ASSERT_leI)
+  subgoal
+    by (auto simp: trail_pol_def dest!: control_stack_length_count_dec)
+  subgoal for a aa ab ac ad b ba ae bb
+    by (auto simp: trail_pol_def control_stack_length_count_dec in_set_take_conv_nth
+        intro!: control_stack_le_length_M control_stack_is_decided
+        dest: control_stack_level_control_stack)
+  done
+
+lemma lit_of_last_trail_pol_lit_of_last_trail_no_CS:
+   \<open>(RETURN o lit_of_last_trail_pol, RETURN o lit_of_hd_trail) \<in>
+         [\<lambda>S. S \<noteq> []]\<^sub>f trail_pol_no_CS \<A> \<rightarrow> \<langle>Id\<rangle>nres_rel\<close>
+  by (auto simp: lit_of_hd_trail_def trail_pol_no_CS_def lit_of_last_trail_pol_def
+     ann_lits_split_reasons_def hd_map rev_map[symmetric] last_rev
+      intro!: frefI nres_relI)
+
 end
